wip

src/Init/Data/Range/Polymorphic/SInt.lean
@@ -13,10 +13,673 @@ import Init.Omega
 public import Init.Data.Range.Polymorphic.BitVec
 import Init.Data.Range.Polymorphic.UInt
 
+import all Init.Data.SInt.Basic
+
 public section
 
 open Std Std.PRange
 
+namespace BitVecModel
+
+open BitVec.Signed
+
+variable {α : Type u} [LE α] [LT α] {β : Type u} [LE β] [LT β]
+
+class HasModel (α : Type u) [LE α] [LT α] (β : outParam (Type v)) [LE β] [LT β]
+    [UpwardEnumerable β] [LawfulUpwardEnumerable β] [LawfulUpwardEnumerableLE β]
+    [LawfulUpwardEnumerableLT β] where
+  encode : α → β
+  decode : β → α
+  encode_decode : encode (decode x) = x
+  decode_encode : decode (encode x) = x
+  le_iff_encode_le : x ≤ y ↔ (encode x) ≤ (encode y)
+  lt_iff_encode_lt : x < y ↔ (encode x) < (encode y)
+
+variable [UpwardEnumerable β] [LawfulUpwardEnumerable β] [LawfulUpwardEnumerableLE β]
+  [LawfulUpwardEnumerableLT β]
+
+scoped instance HasModel.instUpwardEnumerable [m : HasModel α β] :
+    UpwardEnumerable α where
+  succ? a := (succ? (m.encode a)).map m.decode
+  succMany? n a := (succMany? n (m.encode a)).map m.decode
+
+theorem HasModel.succ?_decode [m : HasModel α β] {x : β} :
+    UpwardEnumerable.succ? (m.decode x) = (UpwardEnumerable.succ? x).map m.decode := by
+  simp [instUpwardEnumerable, HasModel.encode_decode]
+
+theorem HasModel.succ?_encode [m : HasModel α β] {x : α} :
+    UpwardEnumerable.succ? (m.encode x) = (UpwardEnumerable.succ? x).map m.encode := by
+  simp [instUpwardEnumerable, Function.comp_def, HasModel.encode_decode]
+
+theorem HasModel.succMany?_decode [m : HasModel α β] {x : β} :
+    UpwardEnumerable.succMany? n' (m.decode x) = (UpwardEnumerable.succMany? n' x).map m.decode := by
+  simp [instUpwardEnumerable, HasModel.encode_decode]
+
+theorem HasModel.succMany?_encode [m : HasModel α β] {x : α} :
+    UpwardEnumerable.succMany? n' (m.encode x) = (UpwardEnumerable.succMany? n' x).map m.encode := by
+  simp [instUpwardEnumerable, Function.comp_def, HasModel.encode_decode]
+
+theorem HasModel.eq_of_encode_eq [m : HasModel α β] (x y : α) :
+    m.encode x = m.encode y → x = y := by
+  sorry
+
+theorem HasModel.encode_inj [m : HasModel α β] {x y : α} :
+    m.encode x = m.encode y ↔ x = y := by
+  exact ⟨m.eq_of_encode_eq x y, by simp +contextual⟩
+
+theorem HasModel.le_iff [m : HasModel α β] {x y : α} :
+    UpwardEnumerable.LE x y ↔ UpwardEnumerable.LE (m.encode x) (m.encode y) := by
+  simp [UpwardEnumerable.le_iff_exists, succMany?_encode, ← Option.map_some,
+    Option.map_inj_right eq_of_encode_eq]
+
+theorem HasModel.lt_iff [m : HasModel α β] {x y : α} :
+    UpwardEnumerable.LT x y ↔ UpwardEnumerable.LT (m.encode x) (m.encode y) := by
+  simp [UpwardEnumerable.lt_iff_exists, succMany?_encode, ← Option.map_some,
+    Option.map_inj_right eq_of_encode_eq]
+
+attribute [local instance] HasModel.instUpwardEnumerable
+scoped instance HasModel.instLawfulUpwardEnumerable [m : HasModel α β] :
+    LawfulUpwardEnumerable α where
+  ne_of_lt x y := by
+    rw [m.lt_iff, ne_eq, ← m.encode_inj]
+    apply LawfulUpwardEnumerable.ne_of_lt
+  succMany?_zero x := by
+    rw [← Option.map_inj_right eq_of_encode_eq, ← succMany?_encode, Option.map_some]
+    apply LawfulUpwardEnumerable.succMany?_zero
+  succMany?_add_one n x := by
+    rw [← Option.map_inj_right eq_of_encode_eq, ← succMany?_encode, Option.map_bind,
+      Function.comp_def]
+    simp only [← succ?_encode]
+    rw [← Function.comp_def, ← Option.bind_map, ← succMany?_encode (n' := n),
+      LawfulUpwardEnumerable.succMany?_add_one]
+
+scoped instance HasModel.instLawfulUpwardEnumerableLE [m : HasModel α β] :
+    LawfulUpwardEnumerableLE α where
+  le_iff x y := by
+    rw [m.le_iff_encode_le, m.le_iff]
+    apply LawfulUpwardEnumerableLE.le_iff
+
+scoped instance HasModel.instLawfulUpwardEnumerableLT [m : HasModel α β] :
+    LawfulUpwardEnumerableLT α where
+  lt_iff x y := by
+    rw [m.lt_iff_encode_lt, m.lt_iff]
+    apply LawfulUpwardEnumerableLT.lt_iff
+instance : Rxc.HasSize Int8 where
+  size lo hi := (hi.toInt + 1 - lo.toInt).toNat
+
+-- theorem rxcHasSize_eq_toBitVec :
+--     Rxc.HasSize.size (Int8.ofBitVec lo) hi = Rxc.HasSize.size lo hi.toBitVec := by
+--   simp [Rxc.HasSize.size, rotate, ← toInt_toBitVec, toInt_eq_ofNat_toNat_rotate_sub]
+--   omega
+
+-- private theorem ofBitVec_eq_iff {x : BitVec 8} {y : Int8} :
+--     Int8.ofBitVec x = y ↔ x = y.toBitVec := by
+--   rw [← toBitVec_ofBitVec x, toBitVec_inj, toBitVec_ofBitVec]
+
+scoped instance instRxcHasSize [m : HasModel α β] [Rxc.HasSize β] :
+    Rxc.HasSize α where
+  size lo hi := Rxc.HasSize.size (m.encode lo) (m.encode hi)
+
+scoped instance instRxcLawfulHasSize [m : HasModel α β] [Rxc.HasSize β] [Rxc.LawfulHasSize β] :
+    Rxc.LawfulHasSize α where
+  size_eq_zero_of_not_le lo hi := by
+    simp only [m.le_iff_encode_le, Rxc.HasSize.size]
+    apply Rxc.LawfulHasSize.size_eq_zero_of_not_le
+  size_eq_one_of_succ?_eq_none lo hi := by
+    simp only [m.le_iff_encode_le, Rxc.HasSize.size,
+      show succ? lo = none ↔ succ? (m.encode lo) = none by simp [m.succ?_encode]]
+    apply Rxc.LawfulHasSize.size_eq_one_of_succ?_eq_none
+  size_eq_succ_of_succ?_eq_some lo hi x := by
+    have : ∀ x, succ? lo = some x ↔ succ? (m.encode lo) = some (m.encode x) := by
+      simp [m.succ?_encode, ← Option.map_some, Option.map_inj_right m.eq_of_encode_eq]
+    simp only [m.le_iff_encode_le, Rxc.HasSize.size, this]
+    apply Rxc.LawfulHasSize.size_eq_succ_of_succ?_eq_some
+
+scoped instance instRxiHasSize [m : HasModel α β] [Rxi.HasSize β] :
+    Rxi.HasSize α where
+  size lo := Rxi.HasSize.size (m.encode lo)
+
+scoped instance instRxiLawfulHasSize [m : HasModel α β] [Rxi.HasSize β] [Rxi.LawfulHasSize β] :
+    Rxi.LawfulHasSize α where
+  size_eq_one_of_succ?_eq_none lo := by
+    have : succ? lo = none ↔ succ? (m.encode lo) = none := by simp [m.succ?_encode]
+    simp only [this, instRxiHasSize]
+    apply Rxi.LawfulHasSize.size_eq_one_of_succ?_eq_none
+  size_eq_succ_of_succ?_eq_some lo lo' := by
+    have : ∀ x, succ? lo = some x ↔ succ? (m.encode lo) = some (m.encode x) := by
+      simp [m.succ?_encode, ← Option.map_some, Option.map_inj_right m.eq_of_encode_eq]
+    simp only [this, instRxiHasSize]
+    apply Rxi.LawfulHasSize.size_eq_succ_of_succ?_eq_some
+
+end BitVecModel
+
+namespace Int8
+
+open BitVec.Signed
+
+attribute [-instance] BitVec.instUpwardEnumerable BitVec.instHasSize BitVec.instHasSize_1
+  BitVec.instHasSize_2 BitVec.instLawfulUpwardEnumerable
+
+instance : UpwardEnumerable Int8 where
+  succ? i := if i + 1 = Int8.minValue then none else some (i + 1)
+  succMany? n i :=
+    have := i.minValue_le_toInt
+    if h : i.toInt + n ≤ Int8.maxValue.toInt then some (.ofIntLE _ (by omega) h) else none
+
+theorem succ?_ofBitVec {x : BitVec 8} :
+    UpwardEnumerable.succ? (Int8.ofBitVec x) = Int8.ofBitVec <$> UpwardEnumerable.succ? x := by
+  simp only [succ?, ← toBitVec_inj, Int8.toBitVec_add, toBitVec_ofBitVec, toBitVec_ofNat,
+    BitVec.ofNat_eq_ofNat, toBitVec_neg, BitVec.reduceNeg, rotate, BitVec.natCast_eq_ofNat,
+    Option.map_eq_map, Option.map_map, Function.comp_def]
+  split <;> split <;> try (simp_all [Int8.add_assoc]; done)
+  all_goals
+    rename_i h h'
+    rw [BitVec.add_assoc, BitVec.add_comm 128#8 1#8, ← BitVec.add_assoc,
+      ← BitVec.eq_sub_iff_add_eq] at h'
+    simp [h] at h'
+
+theorem succMany?_ofBitVec {k : Nat} {x : BitVec 8} :
+    UpwardEnumerable.succMany? k (Int8.ofBitVec x) =
+      Int8.ofBitVec <$> UpwardEnumerable.succMany? k x := by
+  simp only [succMany?, maxValue, ofIntLE_eq_ofInt, ofInt_add, dite_eq_ite, rotate,
+    BitVec.ofNatLT_eq_ofNat, Option.map_eq_map, Option.map_if, ofBitVec_add, ofBitVec_ofNat,
+    ofNat_add, ofNat_bitVecToNat]
+  split <;> split <;> try (simp [← ofBitVec_ofInt, Int8.add_assoc, Int8.add_comm (-128)]; done)
+  all_goals
+    rename_i h h'
+    simp [toInt_eq_ofNat_toNat_rotate_sub, rotate] at h h'
+    omega
+
+theorem upwardEnumerableLE_ofBitVec {x y : BitVec 8} :
+    UpwardEnumerable.LE (Int8.ofBitVec x) (Int8.ofBitVec y) ↔ UpwardEnumerable.LE x y := by
+  simp [UpwardEnumerable.LE, succMany?_ofBitVec, ofBitVec_inj]
+
+theorem upwardEnumerableLT_ofBitVec {x y : BitVec 8} :
+    UpwardEnumerable.LT (Int8.ofBitVec x) (Int8.ofBitVec y) ↔ UpwardEnumerable.LT x y := by
+  simp [UpwardEnumerable.LT, succMany?_ofBitVec, ofBitVec_inj]
+
+instance : LawfulUpwardEnumerable Int8 where
+  ne_of_lt x y := by
+    rw [← ofBitVec_toBitVec x, ← ofBitVec_toBitVec y]
+    simpa [upwardEnumerableLT_ofBitVec, ne_iff_ofBitVec_ne, -ofBitVec_toBitVec] using
+      LawfulUpwardEnumerable.ne_of_lt (α := BitVec 8) _ _
+  succMany?_zero x := by
+    rw [← ofBitVec_toBitVec x]
+    simpa [succMany?_ofBitVec, ofBitVec_inj, -ofBitVec_toBitVec] using succMany?_zero
+  succMany?_add_one n x := by
+    rw [← ofBitVec_toBitVec x]
+    simp [succMany?_ofBitVec, succMany?_add_one, Option.bind_map, Function.comp_def,
+      succ?_ofBitVec, -ofBitVec_toBitVec]
+
+private theorem toBitVec_le {x y : Int8} :
+    x.toBitVec ≤ y.toBitVec ↔ x ≤ y := by
+  rw [Int8.le_iff_toBitVec_sle]
+  simp [LE.le]
+
+private theorem ofBitVec_le {x y : BitVec 8} :
+    Int8.ofBitVec x ≤ Int8.ofBitVec y ↔ x ≤ y := by
+  simp [← toBitVec_le]
+
+instance : LawfulUpwardEnumerableLE Int8 where
+  le_iff x y := by
+    rw [← ofBitVec_toBitVec x, ← ofBitVec_toBitVec y]
+    simpa [upwardEnumerableLE_ofBitVec, -ofBitVec_toBitVec, ofBitVec_le] using
+      LawfulUpwardEnumerableLE.le_iff (α := BitVec 8) _ _
+
+instance : LawfulUpwardEnumerableLT Int8 := inferInstance
+instance : LawfulUpwardEnumerableLT Int8 := inferInstance
+
+instance : Rxc.HasSize Int8 where
+  size lo hi := (hi.toInt + 1 - lo.toInt).toNat
+
+theorem rxcHasSize_eq_toBitVec :
+    Rxc.HasSize.size (Int8.ofBitVec lo) hi = Rxc.HasSize.size lo hi.toBitVec := by
+  simp [Rxc.HasSize.size, rotate, ← toInt_toBitVec, toInt_eq_ofNat_toNat_rotate_sub]
+  omega
+
+private theorem ofBitVec_eq_iff {x : BitVec 8} {y : Int8} :
+    Int8.ofBitVec x = y ↔ x = y.toBitVec := by
+  rw [← toBitVec_ofBitVec x, toBitVec_inj, toBitVec_ofBitVec]
+
+instance : Rxc.LawfulHasSize Int8 where
+  size_eq_zero_of_not_le lo hi := by
+    rw [← ofBitVec_toBitVec lo, ← ofBitVec_toBitVec hi]
+    simpa [rxcHasSize_eq_toBitVec, UInt8.lt_iff_toBitVec_lt, ofBitVec_le, -ofBitVec_toBitVec] using
+      Rxc.LawfulHasSize.size_eq_zero_of_not_le (α := BitVec 8) _ _
+  size_eq_one_of_succ?_eq_none lo hi := by
+    rw [← ofBitVec_toBitVec lo, ← ofBitVec_toBitVec hi]
+    simpa [rxcHasSize_eq_toBitVec, UInt8.le_iff_toBitVec_le, succ?_ofBitVec, ofBitVec_le,
+      -ofBitVec_toBitVec] using Rxc.LawfulHasSize.size_eq_one_of_succ?_eq_none (α := BitVec 8) _ _
+  size_eq_succ_of_succ?_eq_some lo hi x := by
+    rw [← ofBitVec_toBitVec lo, ← ofBitVec_toBitVec x, ← ofBitVec_toBitVec hi]
+    simpa [rxcHasSize_eq_toBitVec, UInt8.le_iff_toBitVec_le, ← UInt8.toBitVec_inj,
+      ofBitVec_le, succ?_ofBitVec, -ofBitVec_toBitVec, ofBitVec_eq_iff] using
+      Rxc.LawfulHasSize.size_eq_succ_of_succ?_eq_some (α := BitVec 8) _ _ _
+
+instance : Rxc.IsAlwaysFinite Int8 := inferInstance
+
+instance : Rxo.HasSize Int8 := .ofClosed
+instance : Rxo.LawfulHasSize Int8 := inferInstance
+instance : Rxo.IsAlwaysFinite Int8 := inferInstance
+
+instance : Rxi.HasSize Int8 where
+  size lo := ((2 : Int) ^ 7 - lo.toInt).toNat
+
+theorem rxiHasSize_eq_toBitVec :
+    Rxi.HasSize.size (Int8.ofBitVec lo) = Rxi.HasSize.size lo := by
+  simp [Rxi.HasSize.size, rotate, toInt_eq_ofNat_toNat_rotate_sub]
+  omega
+
+instance : Rxi.LawfulHasSize Int8 where
+  size_eq_one_of_succ?_eq_none lo := by
+    rw [← ofBitVec_toBitVec lo]
+    simpa [rxiHasSize_eq_toBitVec, succ?_ofBitVec, -ofBitVec_toBitVec] using
+      Rxi.LawfulHasSize.size_eq_one_of_succ?_eq_none (α := BitVec 8) _
+  size_eq_succ_of_succ?_eq_some lo lo' := by
+    rw [← ofBitVec_toBitVec lo, ← ofBitVec_toBitVec lo']
+    simpa [rxiHasSize_eq_toBitVec, succ?_ofBitVec, ofBitVec_eq_iff, -ofBitVec_toBitVec] using
+      Rxi.LawfulHasSize.size_eq_succ_of_succ?_eq_some (α := BitVec 8) _ _
+
+end Int8
+
+namespace Int16
+
+open BitVec.Signed
+
+attribute [-instance] BitVec.instUpwardEnumerable BitVec.instHasSize BitVec.instHasSize_1
+  BitVec.instHasSize_2 BitVec.instLawfulUpwardEnumerable
+
+instance : UpwardEnumerable Int16 where
+  succ? i := if i + 1 = Int16.minValue then none else some (i + 1)
+  succMany? n i :=
+    have := i.minValue_le_toInt
+    if h : i.toInt + n ≤ Int16.maxValue.toInt then some (.ofIntLE _ (by omega) h) else none
+
+theorem succ?_ofBitVec {x : BitVec 16} :
+    UpwardEnumerable.succ? (Int16.ofBitVec x) = Int16.ofBitVec <$> UpwardEnumerable.succ? x := by
+  simp only [succ?, ← toBitVec_inj, Int16.toBitVec_add, toBitVec_ofBitVec, toBitVec_ofNat,
+    BitVec.ofNat_eq_ofNat, toBitVec_neg, BitVec.reduceNeg, rotate, BitVec.natCast_eq_ofNat,
+    Option.map_eq_map, Option.map_map, Function.comp_def]
+  split <;> split <;> try (simp_all [Int16.add_assoc]; done)
+  all_goals
+    rename_i h h'
+    rw [BitVec.add_assoc, BitVec.add_comm 32768#16 1#16, ← BitVec.add_assoc,
+      ← BitVec.eq_sub_iff_add_eq] at h'
+    simp [h] at h'
+
+theorem succMany?_ofBitVec {k : Nat} {x : BitVec 16} :
+    UpwardEnumerable.succMany? k (Int16.ofBitVec x) =
+      Int16.ofBitVec <$> UpwardEnumerable.succMany? k x := by
+  simp only [succMany?, maxValue, ofIntLE_eq_ofInt, ofInt_add, dite_eq_ite, rotate,
+    BitVec.ofNatLT_eq_ofNat, Option.map_eq_map, Option.map_if, ofBitVec_add, ofBitVec_ofNat,
+    ofNat_add, ofNat_bitVecToNat]
+  split <;> split <;> try (simp [← ofBitVec_ofInt, Int16.add_assoc, Int16.add_comm (-32768)]; done)
+  all_goals
+    rename_i h h'
+    simp [toInt_eq_ofNat_toNat_rotate_sub, rotate] at h h'
+    omega
+
+theorem upwardEnumerableLE_ofBitVec {x y : BitVec 16} :
+    UpwardEnumerable.LE (Int16.ofBitVec x) (Int16.ofBitVec y) ↔ UpwardEnumerable.LE x y := by
+  simp [UpwardEnumerable.LE, succMany?_ofBitVec, ofBitVec_inj]
+
+theorem upwardEnumerableLT_ofBitVec {x y : BitVec 16} :
+    UpwardEnumerable.LT (Int16.ofBitVec x) (Int16.ofBitVec y) ↔ UpwardEnumerable.LT x y := by
+  simp [UpwardEnumerable.LT, succMany?_ofBitVec, ofBitVec_inj]
+
+instance : LawfulUpwardEnumerable Int16 where
+  ne_of_lt x y := by
+    rw [← ofBitVec_toBitVec x, ← ofBitVec_toBitVec y]
+    simpa [upwardEnumerableLT_ofBitVec, ne_iff_ofBitVec_ne, -ofBitVec_toBitVec] using
+      LawfulUpwardEnumerable.ne_of_lt (α := BitVec 16) _ _
+  succMany?_zero x := by
+    rw [← ofBitVec_toBitVec x]
+    simpa [succMany?_ofBitVec, ofBitVec_inj, -ofBitVec_toBitVec] using succMany?_zero
+  succMany?_add_one n x := by
+    rw [← ofBitVec_toBitVec x]
+    simp [succMany?_ofBitVec, succMany?_add_one, Option.bind_map, Function.comp_def,
+      succ?_ofBitVec, -ofBitVec_toBitVec]
+
+private theorem toBitVec_le {x y : Int16} :
+    x.toBitVec ≤ y.toBitVec ↔ x ≤ y := by
+  rw [Int16.le_iff_toBitVec_sle]
+  simp [LE.le]
+
+private theorem ofBitVec_le {x y : BitVec 16} :
+    Int16.ofBitVec x ≤ Int16.ofBitVec y ↔ x ≤ y := by
+  simp [← toBitVec_le]
+
+instance : LawfulUpwardEnumerableLE Int16 where
+  le_iff x y := by
+    rw [← ofBitVec_toBitVec x, ← ofBitVec_toBitVec y]
+    simpa [upwardEnumerableLE_ofBitVec, -ofBitVec_toBitVec, ofBitVec_le] using
+      LawfulUpwardEnumerableLE.le_iff (α := BitVec 16) _ _
+
+instance : LawfulUpwardEnumerableLT Int16 := inferInstance
+instance : LawfulUpwardEnumerableLT Int16 := inferInstance
+
+instance : Rxc.HasSize Int16 where
+  size lo hi := (hi.toInt + 1 - lo.toInt).toNat
+
+theorem rxcHasSize_eq_toBitVec :
+    Rxc.HasSize.size (Int16.ofBitVec lo) hi = Rxc.HasSize.size lo hi.toBitVec := by
+  simp [Rxc.HasSize.size, rotate, ← toInt_toBitVec, toInt_eq_ofNat_toNat_rotate_sub]
+  omega
+
+private theorem ofBitVec_eq_iff {x : BitVec 16} {y : Int16} :
+    Int16.ofBitVec x = y ↔ x = y.toBitVec := by
+  rw [← toBitVec_ofBitVec x, toBitVec_inj, toBitVec_ofBitVec]
+
+instance : Rxc.LawfulHasSize Int16 where
+  size_eq_zero_of_not_le lo hi := by
+    rw [← ofBitVec_toBitVec lo, ← ofBitVec_toBitVec hi]
+    simpa [rxcHasSize_eq_toBitVec, UInt16.lt_iff_toBitVec_lt, ofBitVec_le, -ofBitVec_toBitVec] using
+      Rxc.LawfulHasSize.size_eq_zero_of_not_le (α := BitVec 16) _ _
+  size_eq_one_of_succ?_eq_none lo hi := by
+    rw [← ofBitVec_toBitVec lo, ← ofBitVec_toBitVec hi]
+    simpa [rxcHasSize_eq_toBitVec, UInt16.le_iff_toBitVec_le, succ?_ofBitVec, ofBitVec_le,
+      -ofBitVec_toBitVec] using Rxc.LawfulHasSize.size_eq_one_of_succ?_eq_none (α := BitVec 16) _ _
+  size_eq_succ_of_succ?_eq_some lo hi x := by
+    rw [← ofBitVec_toBitVec lo, ← ofBitVec_toBitVec x, ← ofBitVec_toBitVec hi]
+    simpa [rxcHasSize_eq_toBitVec, UInt16.le_iff_toBitVec_le, ← UInt16.toBitVec_inj,
+      ofBitVec_le, succ?_ofBitVec, -ofBitVec_toBitVec, ofBitVec_eq_iff] using
+      Rxc.LawfulHasSize.size_eq_succ_of_succ?_eq_some (α := BitVec 16) _ _ _
+
+instance : Rxc.IsAlwaysFinite Int16 := inferInstance
+
+instance : Rxo.HasSize Int16 := .ofClosed
+instance : Rxo.LawfulHasSize Int16 := inferInstance
+instance : Rxo.IsAlwaysFinite Int16 := inferInstance
+
+instance : Rxi.HasSize Int16 where
+  size lo := ((2 : Int) ^ 15 - lo.toInt).toNat
+
+theorem rxiHasSize_eq_toBitVec :
+    Rxi.HasSize.size (Int16.ofBitVec lo) = Rxi.HasSize.size lo := by
+  simp [Rxi.HasSize.size, rotate, toInt_eq_ofNat_toNat_rotate_sub]
+  omega
+
+instance : Rxi.LawfulHasSize Int16 where
+  size_eq_one_of_succ?_eq_none lo := by
+    rw [← ofBitVec_toBitVec lo]
+    simpa [rxiHasSize_eq_toBitVec, succ?_ofBitVec, -ofBitVec_toBitVec] using
+      Rxi.LawfulHasSize.size_eq_one_of_succ?_eq_none (α := BitVec 16) _
+  size_eq_succ_of_succ?_eq_some lo lo' := by
+    rw [← ofBitVec_toBitVec lo, ← ofBitVec_toBitVec lo']
+    simpa [rxiHasSize_eq_toBitVec, succ?_ofBitVec, ofBitVec_eq_iff, -ofBitVec_toBitVec] using
+      Rxi.LawfulHasSize.size_eq_succ_of_succ?_eq_some (α := BitVec 16) _ _
+
+end Int16
+
+namespace Int32
+
+open BitVec.Signed
+
+attribute [-instance] BitVec.instUpwardEnumerable BitVec.instHasSize BitVec.instHasSize_1
+  BitVec.instHasSize_2 BitVec.instLawfulUpwardEnumerable
+
+instance : UpwardEnumerable Int32 where
+  succ? i := if i + 1 = Int32.minValue then none else some (i + 1)
+  succMany? n i :=
+    have := i.minValue_le_toInt
+    if h : i.toInt + n ≤ Int32.maxValue.toInt then some (.ofIntLE _ (by omega) h) else none
+
+theorem succ?_ofBitVec {x : BitVec 32} :
+    UpwardEnumerable.succ? (Int32.ofBitVec x) = Int32.ofBitVec <$> UpwardEnumerable.succ? x := by
+  simp only [succ?, ← toBitVec_inj, Int32.toBitVec_add, toBitVec_ofBitVec, toBitVec_ofNat,
+    BitVec.ofNat_eq_ofNat, toBitVec_neg, BitVec.reduceNeg, rotate, BitVec.natCast_eq_ofNat,
+    Option.map_eq_map, Option.map_map, Function.comp_def]
+  split <;> split <;> try (simp_all [Int32.add_assoc]; done)
+  all_goals
+    rename_i h h'
+    rw [BitVec.add_assoc, BitVec.add_comm 2147483648#32 1#32, ← BitVec.add_assoc,
+      ← BitVec.eq_sub_iff_add_eq] at h'
+    simp [h] at h'
+
+theorem succMany?_ofBitVec {k : Nat} {x : BitVec 32} :
+    UpwardEnumerable.succMany? k (Int32.ofBitVec x) =
+      Int32.ofBitVec <$> UpwardEnumerable.succMany? k x := by
+  simp only [succMany?, maxValue, ofIntLE_eq_ofInt, ofInt_add, dite_eq_ite, rotate,
+    BitVec.ofNatLT_eq_ofNat, Option.map_eq_map, Option.map_if, ofBitVec_add, ofBitVec_ofNat,
+    ofNat_add, ofNat_bitVecToNat]
+  split <;> split <;> try (simp [← ofBitVec_ofInt, Int32.add_assoc, Int32.add_comm (-2147483648)]; done)
+  all_goals
+    rename_i h h'
+    simp [toInt_eq_ofNat_toNat_rotate_sub, rotate] at h h'
+    omega
+
+theorem upwardEnumerableLE_ofBitVec {x y : BitVec 32} :
+    UpwardEnumerable.LE (Int32.ofBitVec x) (Int32.ofBitVec y) ↔ UpwardEnumerable.LE x y := by
+  simp [UpwardEnumerable.LE, succMany?_ofBitVec, ofBitVec_inj]
+
+theorem upwardEnumerableLT_ofBitVec {x y : BitVec 32} :
+    UpwardEnumerable.LT (Int32.ofBitVec x) (Int32.ofBitVec y) ↔ UpwardEnumerable.LT x y := by
+  simp [UpwardEnumerable.LT, succMany?_ofBitVec, ofBitVec_inj]
+
+instance : LawfulUpwardEnumerable Int32 where
+  ne_of_lt x y := by
+    rw [← ofBitVec_toBitVec x, ← ofBitVec_toBitVec y]
+    simpa [upwardEnumerableLT_ofBitVec, ne_iff_ofBitVec_ne, -ofBitVec_toBitVec] using
+      LawfulUpwardEnumerable.ne_of_lt (α := BitVec 32) _ _
+  succMany?_zero x := by
+    rw [← ofBitVec_toBitVec x]
+    simpa [succMany?_ofBitVec, ofBitVec_inj, -ofBitVec_toBitVec] using succMany?_zero
+  succMany?_add_one n x := by
+    rw [← ofBitVec_toBitVec x]
+    simp [succMany?_ofBitVec, succMany?_add_one, Option.bind_map, Function.comp_def,
+      succ?_ofBitVec, -ofBitVec_toBitVec]
+
+private theorem toBitVec_le {x y : Int32} :
+    x.toBitVec ≤ y.toBitVec ↔ x ≤ y := by
+  rw [Int32.le_iff_toBitVec_sle]
+  simp [LE.le]
+
+private theorem ofBitVec_le {x y : BitVec 32} :
+    Int32.ofBitVec x ≤ Int32.ofBitVec y ↔ x ≤ y := by
+  simp [← toBitVec_le]
+
+instance : LawfulUpwardEnumerableLE Int32 where
+  le_iff x y := by
+    rw [← ofBitVec_toBitVec x, ← ofBitVec_toBitVec y]
+    simpa [upwardEnumerableLE_ofBitVec, -ofBitVec_toBitVec, ofBitVec_le] using
+      LawfulUpwardEnumerableLE.le_iff (α := BitVec 32) _ _
+
+instance : LawfulUpwardEnumerableLT Int32 := inferInstance
+instance : LawfulUpwardEnumerableLT Int32 := inferInstance
+
+instance : Rxc.HasSize Int32 where
+  size lo hi := (hi.toInt + 1 - lo.toInt).toNat
+
+def offset : BitVec 32 := 2 ^ 32 - 1
+
+theorem bla {lo hi : BitVec n} (h : n > 0) :
+    (hi.toInt + 1 - lo.toInt).toNat = (rotate hi).toNat + 1 - (rotate lo).toNat := by
+  match n with
+  | 0 => omega
+  | n + 1 =>
+    simp only [toInt_eq_ofNat_toNat_rotate_sub h, rotate, BitVec.toNat_add, Int.natCast_emod,
+      show ∀ a b c d : Int, (a - b) + c - (d - b) = a + c - d by omega]
+    omega
+
+theorem rxcHasSize_eq_toBitVec :
+    Rxc.HasSize.size (Int32.ofBitVec lo) hi = Rxc.HasSize.size lo hi.toBitVec := by
+  rw [← ofBitVec_toBitVec (x := hi)]
+  generalize hi.toBitVec = hi
+  simp only [Rxc.HasSize.size, toInt_ofBitVec, toBitVec_ofBitVec]
+  apply bla
+
+private theorem ofBitVec_eq_iff {x : BitVec 32} {y : Int32} :
+    Int32.ofBitVec x = y ↔ x = y.toBitVec := by
+  rw [← toBitVec_ofBitVec x, toBitVec_inj, toBitVec_ofBitVec]
+
+instance : Rxc.LawfulHasSize Int32 where
+  size_eq_zero_of_not_le lo hi := by
+    rw [← ofBitVec_toBitVec lo, ← ofBitVec_toBitVec hi]
+    simpa [rxcHasSize_eq_toBitVec, UInt32.lt_iff_toBitVec_lt, ofBitVec_le, -ofBitVec_toBitVec] using
+      Rxc.LawfulHasSize.size_eq_zero_of_not_le (α := BitVec 32) _ _
+  size_eq_one_of_succ?_eq_none lo hi := by
+    rw [← ofBitVec_toBitVec lo, ← ofBitVec_toBitVec hi]
+    simpa [rxcHasSize_eq_toBitVec, UInt32.le_iff_toBitVec_le, succ?_ofBitVec, ofBitVec_le,
+      -ofBitVec_toBitVec] using Rxc.LawfulHasSize.size_eq_one_of_succ?_eq_none (α := BitVec 32) _ _
+  size_eq_succ_of_succ?_eq_some lo hi x := by
+    rw [← ofBitVec_toBitVec lo, ← ofBitVec_toBitVec x, ← ofBitVec_toBitVec hi]
+    simpa [rxcHasSize_eq_toBitVec, UInt32.le_iff_toBitVec_le, ← UInt32.toBitVec_inj,
+      ofBitVec_le, succ?_ofBitVec, -ofBitVec_toBitVec, ofBitVec_eq_iff] using
+      Rxc.LawfulHasSize.size_eq_succ_of_succ?_eq_some (α := BitVec 32) _ _ _
+
+instance : Rxc.IsAlwaysFinite Int32 := inferInstance
+
+instance : Rxo.HasSize Int32 := .ofClosed
+instance : Rxo.LawfulHasSize Int32 := inferInstance
+instance : Rxo.IsAlwaysFinite Int32 := inferInstance
+
+instance : Rxi.HasSize Int32 where
+  size lo := ((2 : Int) ^ 31 - lo.toInt).toNat
+
+theorem rxiHasSize_eq_toBitVec :
+    Rxi.HasSize.size (Int32.ofBitVec lo) = Rxi.HasSize.size lo := by
+  simp [Rxi.HasSize.size, rotate, toInt_eq_ofNat_toNat_rotate_sub]
+  omega
+
+instance : Rxi.LawfulHasSize Int32 where
+  size_eq_one_of_succ?_eq_none lo := by
+    rw [← ofBitVec_toBitVec lo]
+    simpa [rxiHasSize_eq_toBitVec, succ?_ofBitVec, -ofBitVec_toBitVec] using
+      Rxi.LawfulHasSize.size_eq_one_of_succ?_eq_none (α := BitVec 32) _
+  size_eq_succ_of_succ?_eq_some lo lo' := by
+    rw [← ofBitVec_toBitVec lo, ← ofBitVec_toBitVec lo']
+    simpa [rxiHasSize_eq_toBitVec, succ?_ofBitVec, ofBitVec_eq_iff, -ofBitVec_toBitVec] using
+      Rxi.LawfulHasSize.size_eq_succ_of_succ?_eq_some (α := BitVec 32) _ _
+
+end Int32
+namespace Int8
+
+open BitVec.Signed
+
+attribute [-instance] BitVec.instUpwardEnumerable BitVec.instHasSize BitVec.instHasSize_1
+  BitVec.instHasSize_2 BitVec.instLawfulUpwardEnumerable
+
+instance : UpwardEnumerable Int8 where
+  succ? i := if i + 1 = Int8.minValue then none else some (i + 1)
+  succMany? n i :=
+    have := i.minValue_le_toInt
+    if h : i.toInt + n ≤ Int8.maxValue.toInt then some (.ofIntLE _ (by omega) h) else none
+
+theorem succ?_ofBitVec {x : BitVec 8} :
+    UpwardEnumerable.succ? (Int8.ofBitVec x) = Int8.ofBitVec <$> UpwardEnumerable.succ? x := by
+  simp only [succ?, ← toBitVec_inj, Int8.toBitVec_add, toBitVec_ofBitVec, toBitVec_ofNat,
+    BitVec.ofNat_eq_ofNat, toBitVec_neg, BitVec.reduceNeg, rotate, BitVec.natCast_eq_ofNat,
+    Option.map_eq_map, Option.map_map, Function.comp_def]
+  split <;> split <;> try (simp_all [Int8.add_assoc]; done)
+  all_goals
+    rename_i h h'
+    rw [BitVec.add_assoc, BitVec.add_comm 128#8 1#8, ← BitVec.add_assoc,
+      ← BitVec.eq_sub_iff_add_eq] at h'
+    simp [h] at h'
+
+theorem succMany?_ofBitVec {k : Nat} {x : BitVec 8} :
+    UpwardEnumerable.succMany? k (Int8.ofBitVec x) =
+      Int8.ofBitVec <$> UpwardEnumerable.succMany? k x := by
+  simp only [succMany?, maxValue, ofIntLE_eq_ofInt, ofInt_add, dite_eq_ite, rotate,
+    BitVec.ofNatLT_eq_ofNat, Option.map_eq_map, Option.map_if, ofBitVec_add, ofBitVec_ofNat,
+    ofNat_add, ofNat_bitVecToNat]
+  split <;> split <;> try (simp [← ofBitVec_ofInt, Int8.add_assoc, Int8.add_comm (-128)]; done)
+  all_goals
+    rename_i h h'
+    simp [toInt_eq_ofNat_toNat_rotate_sub, rotate] at h h'
+    omega
+
+theorem upwardEnumerableLE_ofBitVec {x y : BitVec 8} :
+    UpwardEnumerable.LE (Int8.ofBitVec x) (Int8.ofBitVec y) ↔ UpwardEnumerable.LE x y := by
+  simp [UpwardEnumerable.LE, succMany?_ofBitVec, ofBitVec_inj]
+
+theorem upwardEnumerableLT_ofBitVec {x y : BitVec 8} :
+    UpwardEnumerable.LT (Int8.ofBitVec x) (Int8.ofBitVec y) ↔ UpwardEnumerable.LT x y := by
+  simp [UpwardEnumerable.LT, succMany?_ofBitVec, ofBitVec_inj]
+
+instance : LawfulUpwardEnumerable Int8 where
+  ne_of_lt x y := by
+    rw [← ofBitVec_toBitVec x, ← ofBitVec_toBitVec y]
+    simpa [upwardEnumerableLT_ofBitVec, ne_iff_ofBitVec_ne, -ofBitVec_toBitVec] using
+      LawfulUpwardEnumerable.ne_of_lt (α := BitVec 8) _ _
+  succMany?_zero x := by
+    rw [← ofBitVec_toBitVec x]
+    simpa [succMany?_ofBitVec, ofBitVec_inj, -ofBitVec_toBitVec] using succMany?_zero
+  succMany?_add_one n x := by
+    rw [← ofBitVec_toBitVec x]
+    simp [succMany?_ofBitVec, succMany?_add_one, Option.bind_map, Function.comp_def,
+      succ?_ofBitVec, -ofBitVec_toBitVec]
+
+private theorem toBitVec_le {x y : Int8} :
+    x.toBitVec ≤ y.toBitVec ↔ x ≤ y := by
+  rw [Int8.le_iff_toBitVec_sle]
+  simp [LE.le]
+
+private theorem ofBitVec_le {x y : BitVec 8} :
+    Int8.ofBitVec x ≤ Int8.ofBitVec y ↔ x ≤ y := by
+  simp [← toBitVec_le]
+
+instance : LawfulUpwardEnumerableLE Int8 where
+  le_iff x y := by
+    rw [← ofBitVec_toBitVec x, ← ofBitVec_toBitVec y]
+    simpa [upwardEnumerableLE_ofBitVec, -ofBitVec_toBitVec, ofBitVec_le] using
+      LawfulUpwardEnumerableLE.le_iff (α := BitVec 8) _ _
+
+instance : LawfulUpwardEnumerableLT Int8 := inferInstance
+instance : LawfulUpwardEnumerableLT Int8 := inferInstance
+
+instance : Rxc.HasSize Int8 where
+  size lo hi := (hi.toInt + 1 - lo.toInt).toNat
+
+theorem rxcHasSize_eq_toBitVec :
+    Rxc.HasSize.size (Int8.ofBitVec lo) hi = Rxc.HasSize.size lo hi.toBitVec := by
+  simp [Rxc.HasSize.size, rotate, ← toInt_toBitVec, toInt_eq_ofNat_toNat_rotate_sub]
+  omega
+
+private theorem ofBitVec_eq_iff {x : BitVec 8} {y : Int8} :
+    Int8.ofBitVec x = y ↔ x = y.toBitVec := by
+  rw [← toBitVec_ofBitVec x, toBitVec_inj, toBitVec_ofBitVec]
+
+instance : Rxc.LawfulHasSize Int8 where
+  size_eq_zero_of_not_le lo hi := by
+    rw [← ofBitVec_toBitVec lo, ← ofBitVec_toBitVec hi]
+    simpa [rxcHasSize_eq_toBitVec, UInt8.lt_iff_toBitVec_lt, ofBitVec_le, -ofBitVec_toBitVec] using
+      Rxc.LawfulHasSize.size_eq_zero_of_not_le (α := BitVec 8) _ _
+  size_eq_one_of_succ?_eq_none lo hi := by
+    rw [← ofBitVec_toBitVec lo, ← ofBitVec_toBitVec hi]
+    simpa [rxcHasSize_eq_toBitVec, UInt8.le_iff_toBitVec_le, succ?_ofBitVec, ofBitVec_le,
+      -ofBitVec_toBitVec] using Rxc.LawfulHasSize.size_eq_one_of_succ?_eq_none (α := BitVec 8) _ _
+  size_eq_succ_of_succ?_eq_some lo hi x := by
+    rw [← ofBitVec_toBitVec lo, ← ofBitVec_toBitVec x, ← ofBitVec_toBitVec hi]
+    simpa [rxcHasSize_eq_toBitVec, UInt8.le_iff_toBitVec_le, ← UInt8.toBitVec_inj,
+      ofBitVec_le, succ?_ofBitVec, -ofBitVec_toBitVec, ofBitVec_eq_iff] using
+      Rxc.LawfulHasSize.size_eq_succ_of_succ?_eq_some (α := BitVec 8) _ _ _
+
+instance : Rxc.IsAlwaysFinite Int8 := inferInstance
+
+instance : Rxo.HasSize Int8 := .ofClosed
+instance : Rxo.LawfulHasSize Int8 := inferInstance
+instance : Rxo.IsAlwaysFinite Int8 := inferInstance
+
+instance : Rxi.HasSize Int8 where
+  size lo := ((2 : Int) ^ 7 - lo.toInt).toNat
+
+theorem rxiHasSize_eq_toBitVec :
+    Rxi.HasSize.size (Int8.ofBitVec lo) = Rxi.HasSize.size lo := by
+  simp [Rxi.HasSize.size, rotate, toInt_eq_ofNat_toNat_rotate_sub]
+  omega
+
+instance : Rxi.LawfulHasSize Int8 where
+  size_eq_one_of_succ?_eq_none lo := by
+    rw [← ofBitVec_toBitVec lo]
+    simpa [rxiHasSize_eq_toBitVec, succ?_ofBitVec, -ofBitVec_toBitVec] using
+      Rxi.LawfulHasSize.size_eq_one_of_succ?_eq_none (α := BitVec 8) _
+  size_eq_succ_of_succ?_eq_some lo lo' := by
+    rw [← ofBitVec_toBitVec lo, ← ofBitVec_toBitVec lo']
+    simpa [rxiHasSize_eq_toBitVec, succ?_ofBitVec, ofBitVec_eq_iff, -ofBitVec_toBitVec] using
+      Rxi.LawfulHasSize.size_eq_succ_of_succ?_eq_some (α := BitVec 8) _ _
+
+end Int8
 namespace Int8
 
 open BitVec.Signed
